coq/NNRC/Optim/NNRCRewrite.v
@@ -95,199 +95,287 @@ Section NNRCRewrite.
     red; simpl; trivial.
   Qed.
 
-  (* {| e3 | $t2 ∈ ♯flatten({| e2 ? ‵{|$t1|} : ‵{||} | $t1 ∈ e1 |}) |}
+
+    (** cNNRC evaluation is only sensitive to the environment modulo
+      lookup. *)
+  Lemma nnrc_core_eval_lookup_equiv_on h σc σ₁ σ₂ (e:nnrc) :
+    lookup_equiv_on (nnrc_free_vars e) σ₁ σ₂ ->
+    nnrc_core_eval h σc σ₁ e = 
+    nnrc_core_eval h σc σ₂ e.
+      Proof.
+        revert σ₁ σ₂.
+        induction e; simpl; intros σ₁ σ₂ eqq; trivial
+        ; try apply lookup_equiv_on_dom_app in eqq.
+        - red in eqq; simpl in eqq; rewrite eqq; tauto.
+        - erewrite IHe1, IHe2; try reflexivity; tauto.
+        - erewrite IHe; try reflexivity; tauto.
+        - destruct eqq as [eqq1 eqq2].
+          rewrite (IHe1 _ _ eqq1).
+          match_destr.
+          erewrite IHe2; try reflexivity.
+          unfold lookup_equiv_on in *.
+          intros; simpl.
+          match_destr.
+          apply eqq2; trivial.
+          apply remove_in_neq; trivial.
+        - destruct eqq as [eqq1 eqq2].
+          rewrite (IHe1 _ _ eqq1).
+          match_destr.
+          destruct d; simpl; trivial.
+          f_equal.
+          apply lift_map_ext; intros.
+          erewrite IHe2; try reflexivity.
+          unfold lookup_equiv_on in *.
+          intros; simpl.
+          match_destr.
+          apply eqq2; trivial.
+          apply remove_in_neq; trivial.
+        - destruct eqq as [eqq1 eqq2].
+          rewrite (IHe1 _ _ eqq1).
+          apply olift_ext; intros.
+          destruct a; simpl; trivial.
+          apply lookup_equiv_on_dom_app in eqq2.
+          destruct eqq2.
+          destruct b; eauto.
+        - destruct eqq as [eqq1 eqq2].
+          rewrite (IHe1 _ _ eqq1).
+          apply olift_ext; intros.
+          apply lookup_equiv_on_dom_app in eqq2.
+          destruct eqq2 as [eqq2 eqq3].
+          destruct a; simpl; trivial.
+          + erewrite IHe2; try reflexivity.
+             unfold lookup_equiv_on in *.
+             intros; simpl.
+             match_destr.
+             apply eqq2; trivial.
+             apply remove_in_neq; trivial.
+          + erewrite IHe3; try reflexivity.
+             unfold lookup_equiv_on in *.
+             intros; simpl.
+             match_destr.
+             apply eqq3; trivial.
+             apply remove_in_neq; trivial.
+      Qed.
+
+  (* {| e3 | $t2 ∈ ♯flatten({| e2 ? ‵{|ee|} : ‵{||} | $t1 ∈ e1 |}) |}
        ≡ ♯flatten({| e2 ? ‵{| LET $t2 := $t1 IN e3 ]|} : ‵{||} | $t1 ∈ e1 |}) *)
 
-  Lemma map_sigma_fusion (e1 e2 e3:nnrc) (v1 v2:var) :
+  Lemma map_sigma_fusion (e1 e2 e3:nnrc) ee (v1 v2:var) :
     ~ In v1 (nnrc_free_vars e3) ->
     nnrc_eq
       (NNRCFor v2 
               (NNRCUnop OpFlatten
                        (NNRCFor v1 e1
-                               (NNRCIf e2 (NNRCUnop OpBag (NNRCVar v1)) (NNRCConst (dcoll nil)))))
+                               (NNRCIf e2 (NNRCUnop OpBag ee) (NNRCConst (dcoll nil)))))
               e3)
       (NNRCUnop OpFlatten
                (NNRCFor v1 e1
                        (NNRCIf e2
-                              (NNRCUnop OpBag (NNRCLet v2 (NNRCVar v1) e3))
+                              (NNRCUnop OpBag (NNRCLet v2 ee e3))
                               (NNRCConst (dcoll nil))))).
   Proof.
     intro notinfree.
     unfold nnrc_eq; intros ? ? ? ? _.
     unfold nnrc_eval; simpl.
     destruct (nnrc_core_eval h cenv env (nnrc_to_nnrc_base e1)); try reflexivity; simpl.
-    dest_eqdec; try congruence.
-    clear e1 e.
-    destruct d; try reflexivity; simpl.
+    destruct d; simpl; trivial.
+    clear e1.
+    repeat rewrite olift_lift.
+    simpl.
+    transitivity (
+        lift dcoll
+             (olift (fun c1 =>
+        (lift_map
+           (fun d1 : data => nnrc_core_eval h cenv ((v2, d1) :: env) (nnrc_to_nnrc_base e3))
+           c1))
+    (olift (fun x : list data => oflatten x)
+      (lift_map
+         (fun d1 : data =>
+          olift
+            (fun d : data =>
+             match d with
+             | dbool true =>
+                 olift (fun d0 : data => Some (dcoll (d0 :: nil)))
+                   (nnrc_core_eval h cenv ((v1, d1) :: env) (nnrc_to_nnrc_base ee))
+             | dbool false => Some (dcoll nil)
+             | _ => None
+             end) (nnrc_core_eval h cenv ((v1, d1) :: env) (nnrc_to_nnrc_base e2))) l)
+                 ))).
+    {
+      match goal with
+        [|- match (olift _ ?x) with | Some _ => _ | None => _ end = _] => destruct x 
+      end; simpl; trivial.
+      destruct (oflatten l0); simpl; trivial.
+    }
+    transitivity (
+      lift dcoll
+           (olift (fun x : list data => oflatten x)
+    (lift_map
+       (fun d1 : data =>
+        olift
+          (fun d : data =>
+           match d with
+           | dbool true =>
+               olift (fun d0 : data => Some (dcoll (d0 :: nil)))
+                 match nnrc_core_eval h cenv ((v1, d1) :: env) (nnrc_to_nnrc_base ee) with
+                 | Some d0 =>
+                     nnrc_core_eval h cenv ((v2, d0) :: (v1, d1) :: env)
+                       (nnrc_to_nnrc_base e3)
+                 | None => None
+                 end
+           | dbool false => Some (dcoll nil)
+           | _ => None
+           end) (nnrc_core_eval h cenv ((v1, d1) :: env) (nnrc_to_nnrc_base e2))) l))).
+    2: { idtac.
+         match goal with
+           [|- _ = olift _ ?x ] => destruct x 
+         end; simpl; trivial.
+         }
+       f_equal.
     induction l; try reflexivity; simpl.
     destruct ((nnrc_core_eval h cenv ((v1, a) :: env) (nnrc_to_nnrc_base e2))); try reflexivity; simpl.
     destruct d; try reflexivity; simpl.
-    case_eq b; intros.
-    - autorewrite with alg.
-      rewrite oflatten_lift_cons_dcoll.
-      autorewrite with alg in IHl.
-      unfold olift in *.
-      case_eq (lift_map
-              (fun d1 : data =>
-               match nnrc_core_eval h cenv ((v1, d1) :: env) (nnrc_to_nnrc_base e2) with
-               | Some (dbool true) =>
-                   match nnrc_core_eval h cenv ((v2, d1) :: (v1, d1) :: env) (nnrc_to_nnrc_base e3) with
-                   | Some x'0 => Some (dcoll (x'0 :: nil))
-                   | None => None
-                   end
-               | Some (dbool false) => Some (dcoll nil)
-               | _ => None
-               end) l); intros; rewrite H1 in IHl; case_eq (lift_map
-                (fun d1 : data =>
-                 match nnrc_core_eval h cenv ((v1, d1) :: env) (nnrc_to_nnrc_base e2) with
-                 | Some (dbool true) => Some (dcoll (d1 :: nil))
-                 | Some (dbool false) => Some (dcoll nil)
-                 | _ => None
-                 end) l); intros; rewrite H2 in IHl; simpl in *.
-      + clear H1 H2.
-        unfold lift in *.
-        case_eq (oflatten l1); case_eq (oflatten l0); intros;  rewrite H1 in *; rewrite H2 in *.
-        * simpl.
-          assert (exists l4, lift_map (fun d1 : data => nnrc_core_eval h cenv ((v2, d1) :: env) (nnrc_to_nnrc_base e3)) l3 = Some l4).
-          destruct (lift_map (fun d1 : data => nnrc_core_eval h cenv ((v2, d1) :: env) (nnrc_to_nnrc_base e3)) l3); try congruence.
-          exists l4; reflexivity.
-          elim H3; clear H3; intros.
-          rewrite H3 in *; clear H3.
-          simpl.
-          inversion IHl. subst; clear IHl.
-          assert (nnrc_core_eval h cenv ((v2, a) :: env) (nnrc_to_nnrc_base e3)
-                  = nnrc_core_eval h cenv((v2, a) :: (v1, a) :: env) (nnrc_to_nnrc_base e3)).
-          rewrite nnrc_to_nnrc_base_free_vars_same in notinfree.
-          generalize (@nnrc_core_eval_remove_free_env _ h cenv ((v2,a)::nil) v1 a env (nnrc_to_nnrc_base e3) notinfree); intros.
-          simpl in H0.
-          rewrite H0; clear H0; reflexivity.
-          rewrite H0; clear H0.
-          destruct (nnrc_core_eval h cenv ((v2, a) :: (v1, a) :: env) (nnrc_to_nnrc_base e3)); try reflexivity.
-          rewrite (oflatten_cons (d::nil) l0 l2).
-          reflexivity.
-          assumption.
-        * simpl.
-          destruct (lift_map (fun d1 : data => nnrc_core_eval h cenv ((v2, d1) :: env) (nnrc_to_nnrc_base e3)) l2); try congruence.
-          simpl.
-          destruct (nnrc_core_eval h cenv ((v2, a) :: env) (nnrc_to_nnrc_base e3)); try reflexivity.
-          destruct (nnrc_core_eval h cenv ((v2, a) :: (v1, a) :: env) (nnrc_to_nnrc_base e3)); try reflexivity.
-          rewrite oflatten_cons_none; [reflexivity|assumption].
-          destruct (nnrc_core_eval h cenv ((v2, a) :: (v1, a) :: env) (nnrc_to_nnrc_base e3)); try reflexivity.
-          rewrite oflatten_cons_none; [reflexivity|assumption].
-        * congruence.
-        * destruct (nnrc_core_eval h cenv ((v2, a) :: (v1, a) :: env) (nnrc_to_nnrc_base e3)); try reflexivity.
-          rewrite oflatten_cons_none; [reflexivity|assumption].
-      + unfold lift in *.
-        case_eq (oflatten l0); intros; rewrite H3 in *; try congruence.
-        destruct (nnrc_core_eval h cenv ((v2, a) :: (v1, a) :: env) (nnrc_to_nnrc_base e3)); try reflexivity.
-        rewrite oflatten_cons_none; [reflexivity|assumption].
-      + unfold lift in *.
-        case_eq (oflatten l0); intros; rewrite H3 in *; try congruence.
-        simpl in *.
-        destruct (nnrc_core_eval h cenv ((v2, a) :: env) (nnrc_to_nnrc_base e3)); try reflexivity.
-        destruct (lift_map (fun d1 : data => nnrc_core_eval h cenv ((v2, d1) :: env) (nnrc_to_nnrc_base e3)) l1); try reflexivity; try congruence.
-        simpl.
-        destruct (nnrc_core_eval h cenv ((v2, a) :: (v1, a) :: env) (nnrc_to_nnrc_base e3)); try reflexivity.
-        destruct (nnrc_core_eval h cenv ((v2, a) :: (v1, a) :: env) (nnrc_to_nnrc_base e3)); try reflexivity.
-        destruct (nnrc_core_eval h cenv ((v2, a) :: (v1, a) :: env) (nnrc_to_nnrc_base e3)); try reflexivity.
-      + destruct (nnrc_core_eval h cenv ((v2, a) :: (v1, a) :: env) (nnrc_to_nnrc_base e3)); try reflexivity.
-    - autorewrite with alg.
-      rewrite oflatten_lift_empty_dcoll.
-      rewrite oflatten_lift_empty_dcoll.
-      autorewrite with alg in IHl.
-      rewrite IHl.
-      reflexivity.
-  Qed.
+    destruct b; intros.
+     - destruct ((nnrc_core_eval h cenv ((v1, a) :: env) (nnrc_to_nnrc_base ee)))
+       ; simpl; trivial.
+       rewrite oflatten_lift_cons_dcoll.
+       rewrite olift_lift; simpl.
+       replace (nnrc_core_eval h cenv ((v2, d) :: (v1, a) :: env) (nnrc_to_nnrc_base e3)) with
+           (nnrc_core_eval h cenv ((v2, d) :: env) (nnrc_to_nnrc_base e3)).
+       2: { idtac.
+            apply nnrc_core_eval_lookup_equiv_on; trivial.
+            red; simpl; intros.
+            destruct (string_eqdec x v2); simpl; trivial.
+            destruct (string_eqdec x v1); simpl; trivial.
+            rewrite nnrc_to_nnrc_base_free_vars_same in notinfree.
+            congruence.
+            }
+       destruct (nnrc_core_eval h cenv ((v2, d) :: env) (nnrc_to_nnrc_base e3))
+        ; simpl; trivial
+        ; [ | match goal with [|- olift _ ?x = _ ] => destruct x; simpl; trivial end].
+        rewrite <- lift_olift.
+        rewrite oflatten_lift_cons_dcoll.
+        f_equal.
+        match type of IHl with
+        | ?x = _ => transitivity x
+        end.
+        + apply olift_ext; trivial.
+        + rewrite IHl.
+           apply olift_ext; trivial.
+ - repeat (rewrite oflatten_lift_empty_dcoll).
+   rewrite (olift_eta oflatten).
+   rewrite IHl.
+   rewrite <- (olift_eta oflatten).
+   trivial.
+            Qed.   
 
-  (* {| e3 | $t2 ∈ ♯flatten({| e2 ? ‵{|$t1|} : ‵{||} | $t1 ∈ e1 |}) |}
-       ≡ ♯flatten({| e2 ? ‵{| LET $t2 := $t1 IN e3 ]|} : ‵{||} | $t1 ∈ e1 |}) *)
+  (* {| e3 | $t2 ∈ ♯flatten({| e2 ? ‵{|ee|} : ‵{||} | $t1 ∈ e1 |}) |}
+       ≡ ♯flatten({| e2 ? ‵{| LET $t1 := ee IN e3 ]|} : ‵{||} | $t1 ∈ e1 |}) *)
 
-  Lemma map_sigma_fusion_samevar (e1 e2 e3:nnrc) (v1:var) :
+  Lemma map_sigma_fusion_samevar (e1 e2 e3:nnrc) e (v1:var) :
     nnrc_eq
       (NNRCFor v1 
               (NNRCUnop OpFlatten
                        (NNRCFor v1 e1
-                               (NNRCIf e2 (NNRCUnop OpBag (NNRCVar v1)) (NNRCConst (dcoll nil)))))
+                               (NNRCIf e2 (NNRCUnop OpBag e) (NNRCConst (dcoll nil)))))
               e3)
       (NNRCUnop OpFlatten
                (NNRCFor v1 e1
                        (NNRCIf e2
-                              (NNRCUnop OpBag e3)
+                              (NNRCUnop OpBag (NNRCLet v1 e e3))
                               (NNRCConst (dcoll nil))))).
   Proof.
     unfold nnrc_eq; intros ? ? ? ? _.
     unfold nnrc_eval; simpl.
     destruct (nnrc_core_eval h cenv env (nnrc_to_nnrc_base e1)); try reflexivity; simpl.
-    dest_eqdec; try congruence.
-    clear e1 e.
-    destruct d; try reflexivity; simpl.
+    destruct d; simpl; trivial.
+    clear e1.
+    repeat rewrite olift_lift.
+    simpl.
+    transitivity (
+        lift dcoll
+             (olift (fun c1 =>
+        (lift_map
+           (fun d1 : data => nnrc_core_eval h cenv ((v1, d1) :: env) (nnrc_to_nnrc_base e3))
+           c1))
+    (olift (fun x : list data => oflatten x)
+      (lift_map
+         (fun d1 : data =>
+          olift
+            (fun d : data =>
+             match d with
+             | dbool true =>
+                 olift (fun d0 : data => Some (dcoll (d0 :: nil)))
+                   (nnrc_core_eval h cenv ((v1, d1) :: env) (nnrc_to_nnrc_base e))
+             | dbool false => Some (dcoll nil)
+             | _ => None
+             end) (nnrc_core_eval h cenv ((v1, d1) :: env) (nnrc_to_nnrc_base e2))) l)
+                 ))).
+    {
+      match goal with
+        [|- match (olift _ ?x) with | Some _ => _ | None => _ end = _] => destruct x 
+      end; simpl; trivial.
+      destruct (oflatten l0); simpl; trivial.
+    }
+    transitivity (
+      lift dcoll
+           (olift (fun x : list data => oflatten x)
+    (lift_map
+       (fun d1 : data =>
+        olift
+          (fun d : data =>
+           match d with
+           | dbool true =>
+               olift (fun d0 : data => Some (dcoll (d0 :: nil)))
+                 match nnrc_core_eval h cenv ((v1, d1) :: env) (nnrc_to_nnrc_base e) with
+                 | Some d0 =>
+                     nnrc_core_eval h cenv ((v1, d0) :: (v1, d1) :: env)
+                       (nnrc_to_nnrc_base e3)
+                 | None => None
+                 end
+           | dbool false => Some (dcoll nil)
+           | _ => None
+           end) (nnrc_core_eval h cenv ((v1, d1) :: env) (nnrc_to_nnrc_base e2))) l))).
+    2: { idtac.
+         match goal with
+           [|- _ = olift _ ?x ] => destruct x 
+         end; simpl; trivial.
+         }
+       f_equal.
     induction l; try reflexivity; simpl.
     destruct ((nnrc_core_eval h cenv ((v1, a) :: env) (nnrc_to_nnrc_base e2))); try reflexivity; simpl.
     destruct d; try reflexivity; simpl.
-    case_eq b; intros.
-    - autorewrite with alg.
-      rewrite oflatten_lift_cons_dcoll.
-      autorewrite with alg in IHl.
-      unfold olift in *.
-      case_eq (lift_map
-              (fun d1 : data =>
-               match nnrc_core_eval h cenv ((v1, d1) :: env) (nnrc_to_nnrc_base e2) with
-               | Some (dbool true) =>
-                   match nnrc_core_eval h cenv ((v1, d1) :: env) (nnrc_to_nnrc_base e3) with
-                   | Some x'0 => Some (dcoll (x'0 :: nil))
-                   | None => None
-                   end
-               | Some (dbool false) => Some (dcoll nil)
-               | _ => None
-               end) l); intros; rewrite H1 in IHl; case_eq (lift_map
-                (fun d1 : data =>
-                 match nnrc_core_eval h cenv ((v1, d1) :: env) (nnrc_to_nnrc_base e2) with
-                 | Some (dbool true) => Some (dcoll (d1 :: nil))
-                 | Some (dbool false) => Some (dcoll nil)
-                 | _ => None
-                 end) l); intros; rewrite H2 in IHl; simpl in *.
-      + clear H1 H2.
-        unfold lift in *.
-        case_eq (oflatten l1); case_eq (oflatten l0); intros;  rewrite H1 in *; rewrite H2 in *.
-        * simpl.
-          assert (exists l4, lift_map (fun d1 : data => nnrc_core_eval h cenv ((v1, d1) :: env) (nnrc_to_nnrc_base e3)) l3 = Some l4).
-          destruct (lift_map (fun d1 : data => nnrc_core_eval h cenv ((v1, d1) :: env) (nnrc_to_nnrc_base e3)) l3); try congruence.
-          exists l4; reflexivity.
-          elim H3; clear H3; intros.
-          rewrite H3 in *; clear H3.
-          simpl.
-          inversion IHl. subst; clear IHl.
-          destruct (nnrc_core_eval h cenv ((v1, a) :: env) (nnrc_to_nnrc_base e3)); try reflexivity.
-          rewrite (oflatten_cons (d::nil) l0 l2).
-          reflexivity.
-          assumption.
-        * simpl.
-          destruct (lift_map (fun d1 : data => nnrc_core_eval h cenv ((v1, d1) :: env) (nnrc_to_nnrc_base e3)) l2); try congruence.
-          simpl.
-          destruct (nnrc_core_eval h cenv ((v1, a) :: env) (nnrc_to_nnrc_base e3)); try reflexivity.
-          rewrite oflatten_cons_none; [reflexivity|assumption].
-        * congruence.
-        * destruct (nnrc_core_eval h cenv ((v1, a) :: env) (nnrc_to_nnrc_base e3)); try reflexivity.
-          rewrite oflatten_cons_none; [reflexivity|assumption].
-      + unfold lift in *.
-        case_eq (oflatten l0); intros; rewrite H3 in *; try congruence.
-        destruct (nnrc_core_eval h cenv ((v1, a) :: env) (nnrc_to_nnrc_base e3)); try reflexivity.
-        rewrite oflatten_cons_none; [reflexivity|assumption].
-      + unfold lift in *.
-        case_eq (oflatten l0); intros; rewrite H3 in *; try congruence.
-        simpl in *.
-        destruct (nnrc_core_eval h cenv ((v1, a) :: env) (nnrc_to_nnrc_base e3)); try reflexivity.
-        destruct (lift_map (fun d1 : data => nnrc_core_eval h cenv ((v1, d1) :: env) (nnrc_to_nnrc_base e3)) l1); try reflexivity; try congruence.
-        simpl.
-        destruct (nnrc_core_eval h cenv ((v1, a) :: env) (nnrc_to_nnrc_base e3)); try reflexivity.
-      + destruct (nnrc_core_eval h cenv ((v1, a) :: env) (nnrc_to_nnrc_base e3)); try reflexivity.
-    - autorewrite with alg.
-      rewrite oflatten_lift_empty_dcoll.
-      rewrite oflatten_lift_empty_dcoll.
-      autorewrite with alg in IHl.
-      rewrite IHl.
-      reflexivity.
-  Qed.
+    destruct b; intros.
+     - destruct ((nnrc_core_eval h cenv ((v1, a) :: env) (nnrc_to_nnrc_base e)))
+       ; simpl; trivial.
+       rewrite oflatten_lift_cons_dcoll.
+       rewrite olift_lift; simpl.
+       replace (nnrc_core_eval h cenv ((v1, d) :: (v1, a) :: env) (nnrc_to_nnrc_base e3)) with
+           (nnrc_core_eval h cenv ((v1, d) :: env) (nnrc_to_nnrc_base e3)).
+       2: { idtac.
+            apply nnrc_core_eval_lookup_equiv_prop; trivial.
+            red; simpl; intros.
+            destruct (string_eqdec x v1); simpl; trivial.
+            }
+       destruct (nnrc_core_eval h cenv ((v1, d) :: env) (nnrc_to_nnrc_base e3))
+        ; simpl; trivial
+        ; [ | match goal with [|- olift _ ?x = _ ] => destruct x; simpl; trivial end].
+        rewrite <- lift_olift.
+        rewrite oflatten_lift_cons_dcoll.
+        f_equal.
+        match type of IHl with
+        | ?x = _ => transitivity x
+        end.
+        + apply olift_ext; trivial.
+        + rewrite IHl.
+           apply olift_ext; trivial.
+ - repeat (rewrite oflatten_lift_empty_dcoll).
+   rewrite (olift_eta oflatten).
+   rewrite IHl.
+   rewrite <- (olift_eta oflatten).
+   trivial.
+            Qed. 
+
 
   Lemma for_over_if x e1 e2  e3 ebody :
     nnrc_eq (NNRCFor x (NNRCIf e1 e2 e3) ebody)
